Cleaning & Renaming

io/Compiler.Model.fst
@@ -36,9 +36,9 @@ val convert_insts : (inst_pi:monitorable_prop) -> (spec_pi:monitorable_prop) -> 
 let convert_insts inst_pi spec_pi c1 cmd_call (cmd:io_cmds) arg = 
   cmd_call cmd arg
 
-(** *** IIO interface **)
+(** **** interfaces **)
 noeq
-type iio_interface = {
+type src_interface = {
   ct : erased tflag -> Type;
   pt : erased tflag -> Type;
 
@@ -53,34 +53,8 @@ type iio_interface = {
   ct_importable : fl:erased tflag -> safe_importable (ct fl) spec_pi ct_rcs fl;
 }
 
-let make_rcs_eff (rcs:tree pck_rc) : typ_posts AllActions rcs =
-  let r : tree (pck_eff_rc AllActions) = map_tree rcs make_rc_eff in
-  assume (equal_trees rcs (map_tree r dfst));
-  r
-
-type ctx_iio (i:iio_interface)  = #fl:erased tflag -> typ_posts fl i.ct_rcs -> typ_io_cmds fl i.inst_pi -> i.ct fl
-
-type prog_iio (i:iio_interface) = #fl:erased tflag -> i.ct (IOActions + fl) -> i.pt (IOActions + fl)
-
-assume val traces_of : #a:Type -> a ^-> trace_property #IO.Sig.event
-
-let iio_language : language = {
-  interface = iio_interface;
-
-  ctx = ctx_iio;
-  pprog = prog_iio;
-  whole = (i:iio_interface & i.pt AllActions);
-
-  link = (fun #i p c -> 
-    (| i, p #AllActions (c #AllActions (make_rcs_eff i.ct_rcs) (inst_io_cmds i.inst_pi)) |));
-  event_typ = IO.Sig.event;
-
-  beh = (on_domain  (i:iio_interface & i.pt AllActions) (fun (| i, w |) -> traces_of w)); 
-}
-
-(** *** ILang interface **)
 noeq
-type ilang_interface = {
+type tgt_interface = {
   ct : erased tflag -> Type u#a;
   pt : Type u#b;
 
@@ -91,25 +65,46 @@ type ilang_interface = {
   //pt_ilang : ilang pt inst_pi;
   ct_ilang : fl:erased tflag -> ilang (ct fl) spec_pi;
 }
+  
+(** **** languages **)
 
-type ctx_ilang (i:ilang_interface) = #fl:erased tflag -> typ_io_cmds fl i.inst_pi -> i.ct fl
-type prog_ilang (i:ilang_interface) = i.ct AllActions -> i.pt
+assume val traces_of : #a:Type -> a ^-> trace_property #IO.Sig.event
 
-let ilang_language : language = {
-  interface = ilang_interface;
+type ctx_src (i:src_interface)  = #fl:erased tflag -> typ_io_cmds fl i.inst_pi -> typ_eff_rcs fl i.ct_rcs -> i.ct fl
+type prog_src (i:src_interface) = #fl:erased tflag -> i.ct (IOActions + fl) -> i.pt (IOActions + fl)
 
-  ctx = ctx_ilang;
-  pprog = prog_ilang;
-  whole = (i:ilang_interface & i.pt);
+let src_language : language = {
+  interface = src_interface;
+
+  ctx = ctx_src;
+  pprog = prog_src;
+  whole = (i:src_interface & i.pt AllActions);
+
+  link = (fun #i p c -> 
+    (| i, p #AllActions (c #AllActions (inst_io_cmds i.inst_pi) (make_rcs_eff i.ct_rcs)) |));
+  event_typ = IO.Sig.event;
+
+  beh = (on_domain _ (fun (| i, w |) -> traces_of w)); 
+}
+
+type ctx_tgt (i:tgt_interface) = #fl:erased tflag -> typ_io_cmds fl i.inst_pi -> i.ct fl
+type prog_tgt (i:tgt_interface) = i.ct AllActions -> i.pt
+
+let tgt_language : language = {
+  interface = tgt_interface;
+
+  ctx = ctx_tgt;
+  pprog = prog_tgt;
+  whole = (i:tgt_interface & i.pt);
 
   link = (fun #i p c -> (| i, p (c #AllActions (inst_io_cmds i.inst_pi)) |));
   event_typ = IO.Sig.event;
 
-  beh = (on_domain  (i:ilang_interface & i.pt) (fun (| i, w |) -> traces_of w)); 
+  beh = (on_domain  (i:tgt_interface & i.pt) (fun (| i, w |) -> traces_of w)); 
 }
 
 (** ** Compile interfaces **)
-let comp_int_iio_ilang (i:iio_interface) : ilang_interface = {
+let comp_int_src_tgt (i:src_interface) : tgt_interface = {
  // pt = resexn i.pt_exportable.etype;
   ct = (fun fl -> (i.ct_importable fl).sitype);
   pt = i.pt AllActions;
@@ -122,9 +117,13 @@ let comp_int_iio_ilang (i:iio_interface) : ilang_interface = {
 }
 
 
-(** ** Phases of compilation **)
-val compiler_pprog_iio_ilang : (#i:iio_interface) -> (p_s:prog_iio i) -> ilang_language.pprog (comp_int_iio_ilang i)
-let compiler_pprog_iio_ilang #i p_s c_t = 
+(** ** Compilation **)
+val backtranslate_ctx : (#i:src_interface) -> (c_t:ctx_tgt (comp_int_src_tgt i)) -> src_language.ctx i
+let backtranslate_ctx #i c_t #fl acts eff_rcs =
+  (i.ct_importable fl).safe_import (c_t #fl acts) eff_rcs
+  
+val compiler_pprog : (#i:src_interface) -> (p_s:prog_src i) -> tgt_language.pprog (comp_int_src_tgt i)
+let compiler_pprog #i p_s c_t = 
   let eff_rcs = make_rcs_eff i.ct_rcs in
   let c_s : i.ct AllActions = (i.ct_importable AllActions).safe_import c_t eff_rcs in
   let p : i.pt AllActions = p_s #AllActions c_s in
@@ -132,48 +131,43 @@ let compiler_pprog_iio_ilang #i p_s c_t =
   // (i.pt_exportable.export eff_rc p)
   p
 
-let phase1 : compiler = {
-  source = iio_language;
-  target = ilang_language;
+let comp : compiler = {
+  source = src_language;
+  target = tgt_language;
 
-  comp_int = comp_int_iio_ilang;
+  comp_int = comp_int_src_tgt;
 
-  compile_pprog = compiler_pprog_iio_ilang;
+  compile_pprog = compiler_pprog;
 
   rel_traces = (==);
 }
 
-val backtranslate : (#i:iio_interface) -> (c_t:ctx_ilang (comp_int_iio_ilang i)) -> iio_language.ctx i
-let backtranslate #i c_t #fl eff_rcs acts =
-  let c_s = (i.ct_importable fl).safe_import (c_t #fl acts) eff_rcs in
-  c_s
-
 (** ** RrHC **)
-let phase1_rrhc_2 (i:iio_interface) (ct:ctx_ilang (comp_int_iio_ilang i)) (ps:prog_iio i) : Lemma (
-  let cs : ctx_iio i = backtranslate #i ct in
-  let it = comp_int_iio_ilang i in
-  let pt : prog_ilang it = (compiler_pprog_iio_ilang #i ps) in
-  traces_of (ps #AllActions (cs #AllActions (make_rcs_eff i.ct_rcs) (inst_io_cmds i.inst_pi))) ==
+let comp_rrhc_2 (i:src_interface) (ct:ctx_tgt (comp_int_src_tgt i)) (ps:prog_src i) : Lemma (
+  let cs : ctx_src i = backtranslate_ctx #i ct in
+  let it = comp_int_src_tgt i in
+  let pt : prog_tgt it = (compiler_pprog #i ps) in
+  traces_of (ps #AllActions (cs #AllActions (inst_io_cmds i.inst_pi) (make_rcs_eff i.ct_rcs))) ==
   traces_of (pt (ct #AllActions (inst_io_cmds it.inst_pi)))) = ()
 
-let phase1_rrhc_1 (i:phase1.source.interface) (ct:phase1.target.ctx (phase1.comp_int i)) (ps:phase1.source.pprog i) : Lemma (
-  let cs : phase1.source.ctx i = backtranslate #i ct in
-  phase1.source.beh (ps `phase1.source.link #i` cs) `phase1.rel_traces` phase1.target.beh (phase1.compile_pprog #i ps `phase1.target.link #(phase1.comp_int i)` ct)) =
-  phase1_rrhc_2 i ct ps
+let comp_rrhc_1 (i:comp.source.interface) (ct:comp.target.ctx (comp.comp_int i)) (ps:comp.source.pprog i) : Lemma (
+  let cs : comp.source.ctx i = backtranslate_ctx #i ct in
+  comp.source.beh (ps `comp.source.link #i` cs) `comp.rel_traces` comp.target.beh (comp.compile_pprog #i ps `comp.target.link #(comp.comp_int i)` ct)) =
+  comp_rrhc_2 i ct ps
   
-let phase1_rrhc_0 (i:phase1.source.interface) (ct:phase1.target.ctx (phase1.comp_int i)) : Lemma (
-      exists (cs:phase1.source.ctx i).
-        forall (ps:phase1.source.pprog i).
-          phase1.source.beh (ps `phase1.source.link #i` cs) `phase1.rel_traces` phase1.target.beh (phase1.compile_pprog #i ps `phase1.target.link #(phase1.comp_int i)` ct)) = 
- introduce exists (cs:phase1.source.ctx i).
-        (forall (ps:phase1.source.pprog i).
-          phase1.source.beh (ps `phase1.source.link #i` cs) `phase1.rel_traces` phase1.target.beh (phase1.compile_pprog #i ps `phase1.target.link #(phase1.comp_int i)` ct)) 
-  with (backtranslate #i ct)
-  and Classical.forall_intro (phase1_rrhc_1 i ct)
+let comp_rrhc_0 (i:comp.source.interface) (ct:comp.target.ctx (comp.comp_int i)) : Lemma (
+      exists (cs:comp.source.ctx i).
+        forall (ps:comp.source.pprog i).
+          comp.source.beh (ps `comp.source.link #i` cs) `comp.rel_traces` comp.target.beh (comp.compile_pprog #i ps `comp.target.link #(comp.comp_int i)` ct)) = 
+ introduce exists (cs:comp.source.ctx i).
+        (forall (ps:comp.source.pprog i).
+          comp.source.beh (ps `comp.source.link #i` cs) `comp.rel_traces` comp.target.beh (comp.compile_pprog #i ps `comp.target.link #(comp.comp_int i)` ct)) 
+  with (backtranslate_ctx #i ct)
+  and Classical.forall_intro (comp_rrhc_1 i ct)
           
-val phase1_rrhc : unit -> Lemma (rrhc phase1)
-let phase1_rrhc () : Lemma (rrhc phase1) by (norm [delta_only [`%rrhc]]) = 
-  Classical.forall_intro_2 (phase1_rrhc_0)
+val comp_rrhc : unit -> Lemma (rrhc comp)
+let comp_rrhc () : Lemma (rrhc comp) by (norm [delta_only [`%rrhc]]) = 
+  Classical.forall_intro_2 (comp_rrhc_0)
 
 
 (** * Tests **)
@@ -210,7 +204,7 @@ let rec ex1_stronger_pis0 (h:trace) (lt:trace) : Lemma
 val ex1_stronger_pis : squash (forall h lt. enforced_locally ex1_inst_pi h lt ==> enforced_locally ex1_spec_pi h lt)
 let ex1_stronger_pis = Classical.forall_intro_2 (Classical.move_requires_2 ex1_stronger_pis0)
 
-let ex1_interface : iio_interface = {
+let ex1_interface : src_interface = {
   spec_pi = ex1_spec_pi;
   inst_pi = ex1_inst_pi;
 
@@ -226,23 +220,22 @@ let ex1_interface : iio_interface = {
   inst_pi_stronger_spec_pi = ex1_stronger_pis;
 }
 
-val ex1_prog : prog_iio ex1_interface
+val ex1_prog : prog_src ex1_interface
 let ex1_prog #fl ctx () : IIO (resexn unit) (fl + IOActions) (fun _ -> True) (fun _ _ _ -> True) =
   let _ = ctx () in
   Inl ()
 
-val ex1_ctx : ctx_iio ex1_interface
-let ex1_ctx #fl eff_rcs io_acts () : IIO (resexn file_descr) fl (fun _ -> True) (ex1_ct_post ()) = 
+val ex1_ctx : ctx_src ex1_interface
+let ex1_ctx #fl io_acts eff_rcs () : IIO (resexn file_descr) fl (fun _ -> True) (ex1_ct_post ()) = 
   io_acts Openfile "/etc/passwd"
 
-val ex1_ctx_t : ctx_ilang (comp_int_iio_ilang ex1_interface)
-let ex1_ctx_t #fl io_acts () : IIOpi (resexn file_descr) fl (comp_int_iio_ilang ex1_interface).spec_pi = 
+val ex1_ctx_t : ctx_tgt (comp_int_src_tgt ex1_interface)
+let ex1_ctx_t #fl io_acts () : IIOpi (resexn file_descr) fl (comp_int_src_tgt ex1_interface).spec_pi = 
   io_acts Openfile "/etc/passwd"
-
 
 (** ** Test 3 - HO 1 **)
 
-let test_ho_interface : iio_interface = {
+let test_ho_interface : src_interface = {
   spec_pi = (fun _ _ _ -> true);
   inst_pi = (fun _ _ _ -> true);
   inst_pi_stronger_spec_pi = ();
@@ -266,13 +259,13 @@ let test_ho_interface : iio_interface = {
 }
 
 
-val test_ho_prog : prog_iio test_ho_interface
+val test_ho_prog : prog_src test_ho_interface
 let test_ho_prog #fl ctx () : IIO (resexn unit) (fl + IOActions) (fun _ -> True) (fun _ _ _ -> True) =
   let _ = ctx (fun fd -> Inl ()) in
   Inl ()
 
-val test_ho_ctx : ctx_iio test_ho_interface
-let test_ho_ctx #fl eff_rcs io_acts cb : IIO (resexn file_descr) fl (fun _ -> True) (fun h rfd lt -> Inl? rfd ==> is_open (Inl?.v rfd) (rev lt @ h)) = 
+val test_ho_ctx : ctx_src test_ho_interface
+let test_ho_ctx #fl io_acts eff_rcs cb : IIO (resexn file_descr) fl (fun _ -> True) (fun h rfd lt -> Inl? rfd ==> is_open (Inl?.v rfd) (rev lt @ h)) = 
   let post1 = root eff_rcs in
   let (| _, pre1 |) = root (left eff_rcs) in 
   let rfd = io_acts Openfile "/etc/passwd" in
